Initial blueprint and formalization.

PartialCombinatoryAlgebras/Basic.lean
@@ -1,3 +1,110 @@
-/-- This is just a test to see if documentation is generated. -/
-structure PartialApplicativeStructure where
-  cow : Nat
+import Mathlib.Data.Part
+
+/-- A partial binary operation on a set. -/
+class PartialApplication (A : Type*) where
+  /-- partial binary application -/
+  app : A → A → Part A
+
+@[inherit_doc]
+infixr:30 "•" => PartialApplication.app
+
+/-- When a set is equipped with a partial application, we allow implicit
+    coercions from the set to its partial elements. -/
+instance PartialApplication.hasCoe {A} [PartialApplication A]: Coe A (Part A) where
+  coe := Part.some
+
+/-- Monadic application that can be used for expressions with nested applications. -/
+@[reducible]
+def PartialApplication.mul {A} [PartialApplication A] (a b : Part A) : Part A :=
+  Part.bind a (fun u => Part.bind b (fun v => app u v))
+
+instance PartialApplication.hasMul {A} [PartialApplication A]: Mul (Part A) where
+  mul := mul
+
+/-- Applicative expressions over a context of variables `Γ` and constants `A`. -/
+inductive Expr (Γ : Type*) (A : Type*) where
+  /-- An element as an expression -/
+| elm : A → Expr Γ A
+  /-- A variable as an expression -/
+| var : Γ → Expr Γ A
+  /-- Formal application of expressions -/
+| app : Expr Γ A → Expr Γ A → Expr Γ A
+
+instance Expr.hasMul {Γ A} : Mul (Expr Γ A) where mul := Expr.app
+
+/-- Applicative expressions equipped with the partial application operation `Expr.app`,
+    which happens to be total. -/
+instance Expr.partialApplication {Γ A : Type*} : PartialApplication (Expr Γ A) where
+  app e₁ e₂ := e₁.app e₂
+
+section Expressions
+
+variable {A : Type*} [PartialApplication A]
+variable {Γ : Type*}
+
+/-- The evaluation of an expression with respect to a partial application
+    and valuation of the variables. -/
+def Expr.eval : Expr Γ A → (Γ → A) → Part A
+| .elm a, _ => a
+| .var x, η => η x
+| .app e₁ e₂, η => do
+  let v₁ ← eval e₁ η
+  let v₂ ← eval e₂ η
+  v₁ • v₂
+
+@[inherit_doc]
+notation " ⟦" e "⟧ " η => Expr.eval e η
+
+/-- The statement that an expression is defined for the given valuation. -/
+def Expr.defined (e : Expr Γ A) (η : Γ → A) := (⟦ e ⟧ η).Dom
+
+@[inherit_doc]
+notation:40 e:40 "↓" η:40 => Expr.defined e η
+
+/-- The statement that an expression is undefined for the given valuation. -/
+def Expr.undefined (e : Expr Γ A) (η : Γ → A) := ¬ (⟦ e ⟧ η).Dom
+
+@[inherit_doc]
+notation e "↑" η:40 => Expr.undefined e η
+
+/-- The left-hand argument of an application is defined if the application is defined. -/
+theorem Expr.defined_left {e₁ e₂ : Expr Γ A} {η : Γ → A} : (e₁.app e₂) ↓ η → e₁ ↓ η := by
+  rintro ⟨_, _⟩
+  assumption
+
+/-- The right-hand argument of an application is defined if the application is defined. -/
+theorem Expr.defined_right {e₁ e₂ : Expr Γ A} {η : Γ → A} : (.app e₁ e₂) ↓ η → (e₂ ↓ η) := by
+  rintro ⟨_, ⟨_, _⟩⟩
+  assumption
+
+end Expressions
+
+/-- The partial combinatory structure on a set `A`. -/
+class PCA (A : Type*) extends PartialApplication A where
+  K : A
+  S : A
+  defined_K₁ : ∀ a, (K • a).Dom
+  defined_S₁ : ∀ a, (S • a).Dom
+  defined_S₂ : ∀ a b, ((S • a).get (defined_S₁ a) • b).Dom
+  eq_K : ∀ (a b : A), (K : Part A) * a * b = a
+  eq_S : ∀ (a b c : A), (S : Part A) * a * b * c = (a * b) * (a * c)
+
+notation "𝕜" => Part.some PCA.K
+notation "𝕤" => Part.some PCA.S
+
+namespace PCA
+
+variable {A : Type*} [PCA A]
+
+lemma definedS (a b : A) : (𝕤 * (a : Part A) * (b : Part A)).Dom := by
+  simp [HMul.hMul, Mul.mul, Part.bind_dom]
+  use (defined_S₁ a)
+  use (defined_S₂ a b)
+
+lemma definedK1 (a : A) : (𝕜 * (a : Part A)).Dom := by
+  simp [HMul.hMul, Mul.mul, Part.bind_dom]
+  use (defined_K₁ a)
+
+def id : A := (𝕤 * 𝕜 * 𝕜 : Part A).get (definedS _ _)
+
+end PCA
